\begin{enumerate}[label=\thesection.\arabic*.,ref=\thesection.\theenumi]
\numberwithin{equation}{enumi}

\item
The state equation and the output equation of a control system are given below : 
\begin{align}
    \vec{\dot X}=\myvec{-4&-1.5\\4&0}\vec{X} + \myvec{4\\0}\vec{U}   
\end{align}
\begin{align}
    \vec{Y} = \myvec{1.5&0.625}\vec{X}
\end{align}
  
Then transfer function representation of the system is 


\item 
\solution
when
\begin{align}
    \vec{\dot{X}} = \vec{A}\vec{X} + \vec{B}\vec{U}
\end{align}
\begin{align}
    \vec{Y} = \vec{C}\vec{X} + \vec{D}\vec{U}
\end{align}
\vskip 0.1cm
where $\vec{A},\vec{B},\vec{C},\vec{D}$ are matrices.
  Then the  transfer  function can be find using
\vskip 0.1cm
\begin{align}
    T(s) = \vec{C}\sbrak{(sI-\vec{A})^{-1}}.\vec{B} + \vec{D}
\end{align}
\vskip 0.1cm
From the given state space representation of the system, we can find matrices as
\begin{align}
    \vec{A}= \myvec{-4&-1.5\\4&0}
\end{align}
\begin{align}
    \vec{B} = \myvec{4\\0}
\end{align}
\begin{align}
     \vec{C} = \myvec{1.5&0.625}
\end{align}
We can find the transfer function using
\begin{align}
    T(s) = \vec{C}\sbrak{(sI-\vec{A})^{-1}}.\vec{B} + \vec{D}
\end{align}
\begin{align}
    (sI - \vec{A}) =  \myvec{s&0\\0&s} -  \myvec{-4&-1.5\\4&0}
\end{align}
\begin{align}
    (sI - \vec{A}) =  \myvec{s-4&-1.5\\4&s}
\end{align}
\begin{align}
    |sI - \vec{A}| = s(s+4) - (-4)\times (-1.5)
\end{align}
\vskip 0.1cm
\begin{align}
    |sI - \vec{A}| = s^2 + 4s+ 6
\end{align}
\vskip 0.1cm
and from (1.2.9)
\begin{align}
    Adj\sbrak{sI - \vec{A}} =  \myvec{s&-1.5\\4&s+4}
\end{align}

\begin{align}
    \sbrak{sI - \vec{A}}^{-1} = \frac{Adj[sI - \vec{A}]}{|sI - \vec{A}|} 
\end{align}
\vskip 0.1cm

  \[ =  \myvec{\frac{s}{(s^2 + 4s + 6)}&\frac{-1.5}{(s^2 + 4s + 6)}\\\frac{4}{(s^2 + 4s + 6)}&\frac{s + 4}{(s^2 + 4s + 6)}}\]
    

\vskip 0.1cm
\begin{align}
    \sbrak{sI - \vec{A}}^{-1}.\vec{B} = \myvec{\frac{s}{(s^2 + 4s + 6)}&\frac{-1.5}{(s^2 + 4s + 6)}\\\frac{4}{(s^2 + 4s + 6)}&\frac{s + 4}{(s^2 + 4s + 6)}}\myvec{4\\0}
\end{align}
\vskip 0.1cm
\begin{align}
    \dot{.\hspace{.095in}.}\hspace{.5in}  \sbrak{sI - \vec{A}}^{-1}.\vec{B} = \myvec{\frac{4s}{(s^2 + 4s + 6)}\\\frac{16}{(s^2 + 4s + 6)}}
\end{align}
\vskip 0.1cm
\begin{align*}
Substituting\,the\,values\,of\,\sbrak{sI - \vec{A}}^{-1}.\vec{B}\,and\,\vec{C}\,in\,equation (1.2.7)   
\end{align*}
\vskip 0.1cm
\begin{align}
     T(s) = \myvec{1.5&0.625}\myvec{\frac{4s}{(s^2 + 4s + 6)}\\\frac{16}{(s^2 + 4s + 6)}}
\end{align}
\vskip 0.1cm
\begin{align}
    T(s) = \myvec{\frac{6s}{(s^2 + 4s + 6)}+\frac{10}{(s^2 + 4s + 6)}}
\end{align}


the transfer function representation of the system is
\vskip 0.1cm
\begin{align}
    \dot{.\hspace{.095in}.}\hspace{.5in}
\bf  T(s) = \myvec{\frac{6s+10}{(s^2 + 4s + 6)}} 
\end{align}
\item

\item 
verify the answer with python code
https://github.com/srikanth2001/EE2227-control-systems/tree/master/codes

\end{enumerate}